Clean up ZKBoo

code/ZKBoo.ec
@@ -88,7 +88,7 @@ module ZKBoo(C : Committer, D : Phi) : SProtocol = {
 
   proc witness_extractor(h : statement, a : message,
                          es : challenge list, z : response list) = {
-    var verified, c, y, cs, ys, i, v, tmp, w, e;
+    var verified, c, y, cs, ys, i, v, tmp, w, e, ret;
     verified <- true;
     (c, y) <- h;
     (ys, cs) <- a;
@@ -100,10 +100,14 @@ module ZKBoo(C : Committer, D : Phi) : SProtocol = {
       verified <- verified /\ tmp;
       i <- i + 1;
     }
-    
-    w <- D.extractor(z);
+    if (fully_consistent z es) {
+      w <- D.extractor(z);
+      ret <- w;
+    } else {
+      ret <- None;
+    }
 
-    return w;
+    return ret;
   }
 
   proc simulator(h : statement, e : challenge) = {
@@ -324,9 +328,6 @@ axiom Com_binding_pr c m1 m2 &m:
 lemma Com_binding :
   phoare[BindingGame(Com).main : true ==> ! res] = binding_prob by bypr=> &m H; smt(Com_binding_pr).
 axiom Com_ll: islossless Com.commit.
-
-axiom bind_three_equiv c1 c2 c3 a1 a1' a2 a2' a3 a3' &m:
-    Pr[BindingGame(Com).bind_three(c1, c2, c3, a1, a1', a2, a2', a3, a3') @ &m : ! res] = binding_prob.
 
 local module Com_Inter = {
   module Corr = Correctness(Com)
@@ -696,116 +697,6 @@ proof.
   by byphoare Com_binding.
 qed.
   
-
-lemma Com_binding_three :
-    phoare[BindingGame(Com).bind_three : true ==> ! res] = binding_prob.
-proof.
-    bypr=> &m Pre.
-    smt(bind_three_equiv).
-qed.
-
-lemma binding_pred_implies_cons c1 c2 c3 m1 m1' m2 m2' m3 m3' &m:
-    Pr[BindingGame(Com).bind_three(c1, c2, c3, m1, m1', m2, m2', m3, m3') @ &m : !res] =
-    Pr[BindingGame(Com).bind_three(c1, c2, c3, m1, m1', m2, m2', m3, m3') @ &m :
-      !(verify m1 c1 /\
-        verify m1' c1 /\
-        verify m2 c2 /\
-        verify m2' c2 /\
-        verify m3 c3 /\
-        verify m3' c3 /\
-        ((m1 = m1') /\ (m2 = m2') /\ (m3 = m3')))].
-proof.
-   byequiv=>//.
-   proc*.
-   inline *. auto.
-qed.
-
-lemma binding_three_cons_pr c1 c2 c3 a1 a1' a2 a2' a3 a3' &m:
-    Pr[BindingGame(Com).bind_three(c1, c2, c3, a1, a1', a2, a2', a3, a3') @ &m :
-      !(verify a1 c1 /\
-        verify a1' c1 /\
-        verify a2 c2 /\
-        verify a2' c2 /\
-        verify a3 c3 /\
-        verify a3' c3 /\
-        ((a1 = a1') /\ (a2 = a2') /\ (a3 = a3')))] = binding_prob.
-proof.
-    have Hbind := bind_three_equiv c1 c2 c3 a1 a1' a2 a2' a3 a3' &m.
-    have <- := Com_binding_pr c1 a1 a1' &m.
-    have <- := binding_pred_implies_cons c1 c2 c3 a1 a1' a2 a2' a3 a3' &m.
-    smt.
-qed.
-
-lemma binding_three_cons c1' c2' c3' a1 a1' a2 a2' a3 a3':
-    islossless BindingGame(Com).bind_three =>
-    phoare[BindingGame(Com).bind_three : c1 = c1' /\ c2 = c2' /\ c3 = c3' /\ m1 = a1 /\ m1' = a1' /\ m2 = a2 /\ m2' = a2' /\ m3 = a3 /\ m3' = a3'
-          ==> !(verify a1 c1' /\
-                verify a1' c1' /\
-                verify a2 c2' /\
-                verify a2' c2' /\
-                verify a3 c3' /\
-                verify a3' c3' /\
-                ((a1 = a1') /\ (a2 = a2') /\ (a3 = a3')))] = binding_prob.
-proof.
-    move=> bg_ll.
-    bypr=> &m Pre.
-    smt(binding_three_cons_pr).
-qed.
-
-lemma Com_binding_three_valid :
-    islossless BindingGame(Com).bind_three =>
-    phoare[BindingGame(Com).bind_three : true ==> res] = (1%r - binding_prob).
-proof.
-    move=> bg_ll.
-    phoare split ! (1%r) binding_prob.
-    proc*. call bg_ll.
-    auto.
-    bypr=> &m Pre.
-    by have <- := bind_three_equiv c1{m} c2{m} c3{m} m1{m} m1'{m} m2{m} m2'{m} m3{m} m3'{m} &m.
-qed.
-
-lemma binding_valid_pred_implies_cons c1 c2 c3 m1 m1' m2 m2' m3 m3' &m:
-    Pr[BindingGame(Com).bind_three(c1, c2, c3, m1, m1', m2, m2', m3, m3') @ &m : res] =
-    Pr[BindingGame(Com).bind_three(c1, c2, c3, m1, m1', m2, m2', m3, m3') @ &m :
-       (verify m1 c1 /\
-        verify m1' c1 /\
-        verify m2 c2 /\
-        verify m2' c2 /\
-        verify m3 c3 /\
-        verify m3' c3 /\
-        ((m1 = m1') /\ (m2 = m2') /\ (m3 = m3')))].
-proof.
-   byequiv=>//.
-   proc*.
-   inline *. auto.
-qed.
-
-lemma binding_three_cons_valid c1' c2' c3' a1 a1' a2 a2' a3 a3':
-    islossless BindingGame(Com).bind_three =>
-    phoare[BindingGame(Com).bind_three : c1 = c1' /\ c2 = c2' /\ c3 = c3' /\ m1 = a1 /\ m2 = a2 /\ m3 = a3 /\ m1' = a1' /\ m2' = a2' /\ m3' = a3'
-           ==> (verify a1 c1' /\
-                verify a1' c1' /\
-                verify a2 c2' /\
-                verify a2' c2' /\
-                verify a3 c3' /\
-                verify a3' c3' /\
-                ((a1 = a1') /\ (a2 = a2') /\ (a3 = a3')))] = (1%r - binding_prob).
-proof.
-    move=> bg_ll.
-    phoare split ! (1%r) binding_prob.
-    proc.
-    call (:true).
-    auto.
-    call (:true).
-    auto.
-    call (:true).
-    auto. auto.
-
-    have Hvalid := binding_three_cons c1' c2' c3' a1 a1' a2 a2' a3 a3' bg_ll.
-    proc*. call Hvalid.
-    auto.
-qed.
-
 local module SHVZK_Inter = {
     module ZK = ZKBoo(Com, Decomp)
     module PZK = Privacy(Decomp)
@@ -907,7 +798,6 @@ proof.
     call (:true). auto.
     while (={valid_com} /\ e1{1} = e{2} /\ cs0{1} = cs{2} /\ i{2} = i0{1} /\ ws{1} = vs{2}). sim.
     auto. progress.
-    (* fission{1} 9 @ 2,4. *)
     while (={i, cs, glob Com} /\
            forall i, (if (in_dom_f n e{2} i) then (nth witness ZKBoo.ws{1} i = nth witness vs{2} (proj_mapping i e{2})) else true)).
     - if{2}.
@@ -960,7 +850,6 @@ proof.
   - auto; smt().
   auto.
   while (={cs, i, glob Com, vs, e}).
-           (* forall i, (if (in_dom_f n e{1} i) then (nth_looping vs{1} (i) = nth_looping vs{2} i) else true)). *)
   - if{1}.
     + auto.
       call (:true).
@@ -973,26 +862,6 @@ proof.
   auto; progress.
 qed.
 
-  (* proc verify(h : statement, m : message, e : challenge, z : response) = { *)
-  (*   var ws, i, view, com, ys, cs, c, y, valid_com, valid; *)
-  (*   (c, y) <- h; *)
-  (*   (ys, cs) <- m; *)
-  (*   ws <- f_inv z; *)
-  (*   i <- 0; *)
-  (*   valid_com <- true; *)
-  (*   while (i < n) { *)
-  (*     if (in_dom_f n e i) { *)
-  (*       view <- nth witness ws (proj_mapping i e); *)
-  (*       com <- nth witness cs i; *)
-  (*       valid_com <- valid_com /\ (verify view com) /\ nth witness ys i = output view; *)
-  (*     } *)
-  (*     i <- i + 1; *)
-  (*   } *)
-  (*   valid <- D.verify(c, z, e, ys); *)
-
-  (*   return valid_com /\ valid /\ reconstruct ys = y; *)
-
-  (* } *)
 
 local module SoundnessInter = {
   module ZK = ZKBoo(Com, Decomp)
@@ -1004,7 +873,7 @@ local module SoundnessInter = {
     (ys, cs) <- m;
     q <- 0;
     valid <- true;
-    while (q < n) {
+    while (q < size zs) {
       e <- nth witness es q;
       ver <- ZK.verify(h, m , e, nth witness zs q);
       valid <- valid /\ ver;
@@ -1049,12 +918,6 @@ local module SoundnessInter = {
     return (undup es = es) /\ v /\ w;
   }
 }.
-
-local equiv soundness_inter :
-  Sigma.SpecialSoundness(ZKBoo(Com, Decomp)).main ~ SoundnessInter.main :
-  ={h, m} /\ c{1} = es{2} /\ z{1} = vs{2} ==> ={res}.
-proof.
-admitted.
 
 local lemma consistent_views h' a es' vs':
     0 < size es'  /\
@@ -1170,7 +1033,7 @@ proof.
     + progress; smt().
     + auto; smt().
     + progress; smt().
-  while (h = h' /\ m = a /\ es = es' /\ zs = vs' /\ 0 <= q /\ valid) (n - q); auto.
+  while (h = h' /\ m = a /\ es = es' /\ zs = vs' /\ 0 <= q /\ valid) (size zs - q); auto.
   - exists* q; elim*=>q.
     have Hver := H9 q.
     call Hver.
@@ -1222,17 +1085,125 @@ proof.
   smt(f_inv_hom).
   smt.
 qed.
-  
 
-(* NOTE: Properties needed... *)
-(* (forall i, 0 <= i < n => phoare[Phi.verify : c = c' /\ vs = nth witness vs'' i /\ e = i /\ ys = ys' /\ e \in challenge ==> res] = 1%r) /\ *)
-(* size vs'' = size es /\ es = [0;1;2]  /\ *)
-(* (forall i, 0 <= i < size es' => nth witness es' i \in challenge) /\ *)
-(* valid_circuit c' /\ *)
-(* fully_consistent vs'' es /\ size ys' = size vs'' /\ *)
-
+local lemma soundness_inter:
+    equiv[Sigma.SpecialSoundness(ZKBoo(Com, Decomp)).main ~ SoundnessInter.main :
+          ={h, m, glob Decomp} /\ size es{2} = size vs{2} /\ h{2}.`2 = reconstruct m{2}.`1 /\ c{1} = es{2} /\ z{1} = vs{2} /\ es{2} <> [] ==> ={res}].
+proof.
+    proc.
+    inline *.
+    auto.
+    sp.
+    case (fully_consistent vs{2} es{2}).
+    rcondt{2} 12; progress.
+    - auto.
+      while (true); auto.
+      while (true); auto.
+      while (true); auto.
+    rcondt{1} 11.
+    - auto.
+      while (true); auto.
+      while (true); auto.
+    auto.
+    call (:true).
+    swap{1} 2 -1.
+    sp. auto.
+    while (h1{1} = h{1} /\ z1{1} = vs{2} /\ vs'{2} = vs{2} /\ ={verified, c1, glob Decomp} /\ i0{1} = i{2} /\ es{1} = es1{2} /\ ys0{1} = ys1{2}).
+    - auto.
+      call (:true).
+      auto; progress.
+    auto.
+    while{2} (={glob Decomp}) (size es0{2} - l{2}); auto.
+    while (true) (size es0 - k); auto.
+    inline *. if.
+    while (true) (n - j); auto.
+    - progress. smt().
+    - progress. smt().
+    - smt().
+    - skip. smt().
+    - progress. smt().
+    smt().
+    auto.
+    while (h{1} = (c{2}, reconstruct ys{2}) /\ valid_all{1} = valid{2} /\ ={glob Decomp} /\ 0 <= q{2} <= size zs{2} /\ size zs{2} = size es0{2}
+                                   /\ drop q{2} zs{2} = z_copy{1}
+                                   /\ drop q{2} es0{2} = c_copy{1}
+                                   /\ m{1} = m0{2} /\ c{2} = h0{2}.`1 /\ h0{2}.`2 = reconstruct ys{2}).
+    auto.
+    call (:true).
+    while (={valid_com, ws, glob Decomp} /\ i{1} = i0{2} /\ e{1} = e3{2} /\ cs{1} = cs1{2}).
+    - auto; progress.
+    auto; progress.
+    - smt(drop_nth). 
+      smt(drop_nth).
+      smt(drop_nth).
+      smt(drop_nth).
+      smt(drop_nth).
+      smt(drop_nth).
+      smt(drop_nth).
+      smt.
+      smt.
+      smt.
+    skip; progress.
+    smt(size_ge0).
+    smt(size_ge0).
+    smt(size_ge0).
+    smt(size_ge0).
+    smt(size_ge0).
+    smt(size_ge0).
+    smt(n_pos).
+    rcondf{2} 12; progress.
+    - while (true); auto.
+      while (true); auto.
+      while (true); auto.
+    rcondf{1} 11; progress.
+    - while (true); auto.
+      while (true); auto.
+    auto.
+    while (h1{1} = h{1} /\ z1{1} = vs{2} /\ vs'{2} = vs{2} /\ ={verified, c1, glob Decomp} /\ i0{1} = i{2} /\ es{1} = es1{2} /\ ys0{1} = ys1{2}).
+    - auto.
+      call (:true).
+      auto; progress.
+    auto.
+    while{2} (true) (size es0{2} - l{2}); auto.
+    - while (true) (size es0 - k); auto.
+      if. auto.
+      while (true) (n - j); auto.
+      + progress. smt().
+      + progress. smt().
+        smt().
+      skip.
+      smt().
+      smt().
+    while (h{1} = (c{2}, reconstruct ys{2}) /\ valid_all{1} = valid{2} /\ ={glob Decomp} /\ 0 <= q{2} <= size zs{2} /\ size zs{2} = size es0{2}
+                                   /\ drop q{2} zs{2} = z_copy{1}
+                                   /\ drop q{2} es0{2} = c_copy{1}
+                                   /\ m{1} = m0{2} /\ c{2} = h0{2}.`1 /\ h0{2}.`2 = reconstruct ys{2}).
+    auto.
+    call (:true).
+    while (={valid_com, ws, glob Decomp} /\ i{1} = i0{2} /\ e{1} = e3{2} /\ cs{1} = cs1{2}).
+    - auto; progress.
+    auto; progress.
+    smt(drop_nth).
+    smt(drop_nth).
+    smt(drop_nth).
+    smt(drop_nth).
+    smt(drop_nth).
+    smt(drop_nth).
+    smt(drop_nth).
+    smt(drop_nth).
+    smt.
+    smt.
+    skip; progress.
+    smt(size_ge0).
+    smt(size_ge0).
+    smt.
+    smt.
+    smt(size_ge0).
+    smt(size_ge0).
+qed.
+ 
 axiom decomp_soundness c' vs'' (es' : challenge list) ys':
-    (forall i, 0 <= i < n => phoare[Decomp.verify : c = c' /\ vs = nth witness vs'' i /\ e = i /\ ys = ys' /\ e \in challenge ==> res] = 1%r) =>
+    (forall i, 0 <= i < size es' => phoare[Decomp.verify : c = c' /\ vs = nth witness vs'' i /\ ys = ys' /\ e = nth witness es' i ==> res] = 1%r) =>
     (* (forall i, 0 <= i < n => in_doms_f n es i) (* Must reveal all views *) => *)
     phoare[Soundness(Decomp).main :
       size vs'' = size es' /\ undup es' = es' /\ size es' = 3 /\ es' = [0;1;2] /\
@@ -1263,7 +1234,7 @@ proof.
   - smt().
   - skip. smt().
   - smt().
-  while (h = h' /\ m = a /\ es = es' /\ zs = vs' /\ valid) (n - q); auto.
+  while (h = h' /\ m = a /\ es = es' /\ zs = vs' /\ valid) (size zs - q); auto.
   exists* q; elim*=> q.
   have Hver := H9 q.
   call Hver.
@@ -1284,7 +1255,7 @@ proof.
   - smt().
   - skip. smt().
   - smt().
-  while (h = h' /\ m = a /\ es = es' /\ zs = vs' /\ valid) (n - q); auto.
+  while (h = h' /\ m = a /\ es = es' /\ zs = vs' /\ valid) (size zs - q); auto.
   exists* q; elim*=> q.
   have Hver := H9 q.
   call Hver.
@@ -1310,7 +1281,7 @@ proof.
   - smt().
   - skip. smt().
   - smt().
-  while (h = h' /\ m = a /\ es = es' /\ zs = vs' /\ valid) (n - q); auto.
+  while (h = h' /\ m = a /\ es = es' /\ zs = vs' /\ valid) (size zs - q); auto.
   exists* q; elim*=> q.
   have Hver := H9 q.
   call Hver.
@@ -1322,10 +1293,69 @@ proof.
   - smt().
 qed.
 
-lemma soundness s h' a (vs' : response list) es' &m:
+lemma sigma_le_decomp (Decomp <: D.Phi) (Com <: Commit.Committer) c' y' ys' cs' e' z' &m:
+    Pr[ZKBoo(Com, Decomp).verify((c', y'), (ys', cs'), e', z') @ &m : res] <= Pr[Decomp.verify(c', z', e', ys') @ &m : res].
+proof.
+  byequiv=>//.
+  proc*.
+  inline ZKBoo(Com, Decomp).verify.
+  auto.
+  call (:true).
+  auto.
+  while{1} (true) (n - i{1}).
+  - progress.
+  - auto; progress.
+    + smt().
+  auto; progress.
+  smt().
+qed.
+
+lemma verify_decomp (Decomp <: D.Phi) (Com <: Commit.Committer) c' y' ys' cs' e' z' &m:
+    Pr[ZKBoo(Com, Decomp).verify((c', y'), (ys', cs'), e', z') @ &m : res] = 1%r =>
+    Pr[Decomp.verify(c', z', e', ys') @ &m : res] = 1%r.
+proof.
+  progress. 
+  move: H.
+  apply contraLR. 
+  progress.
+  have : Pr[Decomp.verify(c', z', e', ys') @ &m : res] < 1%r by smt.
+  clear H; move => Hdecomp.
+  have -> :
+    Pr[ZKBoo(Com, Decomp).verify((c', y'), (ys', cs'), e', z') @ &m : res] < 1%r =>
+    Pr[ZKBoo(Com, Decomp).verify((c', y'), (ys', cs'), e', z') @ &m : res] <> 1%r by smt.
+  progress.
+  have Hrel := sigma_le_decomp Decomp Com c' y' ys' cs' e' z' &m.
+  have :
+    Pr[Decomp.verify(c', z', e', ys') @ &m : res] < 1%r =>
+    Pr[ZKBoo(Com, Decomp).verify((c', y'), (ys', cs'), e', z') @ &m : res] < 1%r by smt().
+  clear Hrel; move=> Hrel.
+  by have := Hrel Hdecomp.
+  trivial.
+qed.
+
+lemma verify_decomp_phoare c' y' ys' cs' e' z':
+    phoare[ZKBoo(Com, Decomp).verify : h = (c' , y') /\ m = (ys', cs') /\ e = e' /\ z = z' ==> res] = 1%r =>
+    phoare[Decomp.verify : c = c' /\ vs = z' /\ e = e' /\ ys = ys' ==> res] = 1%r.
+proof.
+   have ->:
+    phoare[ZKBoo(Com, Decomp).verify : h = (c', y') /\ m = (ys', cs') /\ e = e' /\ z = z' ==> res] = 1%r <=>
+    (forall &m, Pr[ZKBoo(Com, Decomp).verify((c', y'), (ys', cs'), e', z') @ &m : res] = 1%r).
+   progress.
+   byphoare H=>//.
+   bypr=>//. progress.
+   have := H &m. smt().
+   have H := verify_decomp Decomp Com c' y' ys' cs' e' z'.
+   progress. 
+   bypr=> &m Pre.
+   have H' := H &m.
+   smt().
+qed.
+
+lemma soundness s h' (a : message) (vs' : response list) es' &m:
     0 < s /\ size es' = s /\ size vs' = size es' /\ valid_circuit (fst h') /\
-    (exists a b i, 0 <= a < size es' && 0 <= b < size es' && 0 <= i < n && a <> b /\ in_dom_f n (nth witness es' a) i /\ in_dom_f n (nth witness es' b) i)  /\
+    (exists a b i', 0 <= a < size es' && 0 <= b < size es' && 0 <= i' < n && a <> b /\ in_dom_f n (nth witness es' a) i' /\ in_dom_f n (nth witness es' b) i')  /\
     es' = undup es' /\ (forall i, 0 <= i < size es' => nth witness es' i \in challenge) /\
+    h'.`2 = reconstruct a.`1 /\ 
     (forall i,
       phoare[ZKBoo(Com, Decomp).verify :
         0 <= i < size es' =>
@@ -1337,24 +1367,119 @@ proof.
     Pr[SpecialSoundness(ZKBoo(Com, Decomp)).main(h', a, es', vs') @ &m : res] =
     Pr[SoundnessInter.main(h', a, es', vs') @ &m : res].
   byequiv soundness_inter=>//.
-  byphoare(: h = h' /\ m = a /\ es = es' /\ vs = vs' ==> _)=>//.
+  progress; smt().
+  byphoare(: h = h' /\ m = (a.`1, a.`2) /\ es = es' /\ vs = vs' ==> _)=>//.
   proc.
   sp; auto.
   seq 1 : (#pre /\ v /\ fully_consistent vs' es') (1%r - binding_prob) 1%r (binding_prob) 0%r (#pre /\ v).
   - inline *.
     auto.
-    while (true); auto.
-    while (valid); auto.
-    call (:true).
-    while (valid_com); auto.
-    + progress.
-    admit.
-    admit.
+    while (true); sp; auto.
+    while (valid /\ es0 = es' /\ zs = vs' /\ h0 = h /\ h = h' /\ m = m0 /\ m = (a.`1, a.`2)); auto.
+    exists* q. elim*=>q.
+    have Dver := verify_decomp_phoare h'.`1 h'.`2 a.`1 a.`2 (nth witness es' q) (nth witness vs' q).
+    have Hver := H14 q.
+    have : phoare[ ZKBoo(Com, Decomp).verify :
+               h = (h'.`1, h'.`2) /\
+               m = (a.`1, a.`2) /\
+               e = nth witness es' q /\ z = nth witness vs' q ==> res] = 1%r.
+    - conseq (: 0 <= q && q < size es' => h = (h'.`1, h'.`2) /\
+                m = (a.`1, a.`2) /\ e = nth witness es' q /\ z = nth witness vs' q
+              ==> _).
+    smt().
+    proc*. call Hver.
+    auto. smt().
+    clear Hver; move=> Hver.
+    have := Dver Hver.
+    clear Dver; move=> Dver.
+    have Dver' : hoare[ Decomp.verify :
+                  c = h'.`1 /\
+                  vs = nth witness vs' q /\ e = nth witness es' q /\ ys = a.`1 ==>
+                  res].
+    - hoare.
+      phoare split ! 1%r 1%r.
+      + progress.
+        proc*. call Dver.
+        auto. smt().
+    call Dver'.
+    clear Dver Dver' Hver.
+    splitwhile 11 : (i < n - 1).
+    seq 11 : (#pre /\ c1 = h.`1 /\ h = h' /\ valid_com /\ i = n - 1 /\ e0 = nth witness es0 q /\ z = nth witness zs q /\ ys1 = a.`1 /\ ws = f_inv z /\ m = (ys1, cs1) /\ m = a /\ reconstruct a.`1 = y1).
+    while (0 <= i < n /\ h = h' /\ q < size zs /\ ws = f_inv z /\ m = (ys1, cs1) /\ a = m /\ e0 = nth witness es0 q /\ es0 = es' /\ z = nth witness zs q /\ zs = vs' /\ valid_com); auto. 
+    + progress. 
+      smt().
+      smt().
+      have PrVer := verify_commitments_phoare h{hr} (ys1{hr}, cs1{hr}) (nth witness es0{hr} q) (nth witness zs{hr} q).
+      have := H14 q. clear H14=> H14.
+      move: PrVer H14 H18.
+      pose e' := (nth witness es0{hr} q).
+      pose z' := (nth witness zs{hr} q).
+      pose ys' := ys1{hr}.
+      pose cs' := cs1{hr}.
+      pose es' := es0{hr}.
+      pose h' := h{hr}.
+      move=> PrVer Hver Hdom.
+      have : phoare[ ZKBoo(Com, Decomp).verify :
+                     h = h' /\ m = (ys', cs') /\ e = e' /\ z = z' ==>
+                     res] = 1%r.
+      - conseq Hver; progress.
+      clear Hver; move=> Hver.
+      have := PrVer Hver i{hr} _. smt().
+      clear PrVer; move=> PrVer.
+      apply PrVer.
+      smt().
+      smt().
+      progress.
+      + smt().
+      + smt().
+      + smt().
+      + smt().
+      + smt().
+    rcondt 1.
+    - skip; progress.
+      + smt().
+    rcondf 3.
+    - wp; skip; progress.
+    if.
+    - auto; progress.
+      have PrVer := verify_commitments_phoare h{hr} a (nth witness es0{hr} q{hr}) (nth witness zs{hr} q{hr}).
+      have := H14 q{hr}. clear H14=> H14.
+      move: PrVer H14 H18.
+      pose e' := (nth witness es0{hr} q{hr}).
+      pose z' := (nth witness zs{hr} q{hr}).
+      pose ys' := ys1{hr}.
+      pose cs' := cs1{hr}.
+      pose es' := es0{hr}.
+      pose h' := h{hr}.
+      move=> PrVer Hver Hdom.
+      have : phoare[ ZKBoo(Com, Decomp).verify :
+                     h = h' /\ m = a /\ e = e' /\ z = z' ==>
+                     res] = 1%r.
+      - conseq Hver; progress. 
+      clear Hver; move=> Hver.
+      have := PrVer Hver (n-1) _. smt().
+      clear PrVer; move=> PrVer.
+      apply PrVer.
+    auto.
   - have ConsViews := pr_not h' a es' vs' _.
     + progress.
       smt().
-    by call ConsViews.
-  have Dsound := decomp_soundness (fst h') vs' es' (fst a) _. admit.
+    call ConsViews.
+    skip; progress.
+    smt().
+  have Dsound := decomp_soundness (fst h') vs' es' (fst a) _. 
+  - progress.
+    have := H14 i=> Sver.
+    have Dver := verify_decomp_phoare h'.`1 h'.`2 a.`1 a.`2 (nth witness es' i) (nth witness vs' i).
+    have : phoare[ ZKBoo(Com, Decomp).verify :
+                   h = (h'.`1, h'.`2) /\
+                   m = (a.`1, a.`2) /\
+                   e = nth witness es' i /\ z = nth witness vs' i ==> res] = 1%r.
+    conseq Sver. smt().
+    clear Sver; move=> Sver.
+    have Dver' := Dver Sver.
+    conseq Dver'.
+    progress.
   call Dsound.
   skip; progress.
   smt().
@@ -1366,416 +1491,8 @@ proof.
   auto.
   while (true); auto.
   + progress.
-qed.
-  
-  
-  
-local lemma extraction_success
-      c' y y1 y2 y3 c1 c2 c3
-      w1 w2 w3 w1' w2' w3'
-      k1 k2 k3 k1' k2' k3':
-  islossless BindingGame(Com).bind_three =>
-  phoare[ZKBoo(Com).verify :
-      h = (c',y) /\ m = (y1,y2,y3,c1,c2,c3) /\ z = (k1, w1, k2, w2) ==>
-      res /\ valid_output_shares y y1 y2 y3 /\ valid_view 1 w1 w2 c' k1 k2 /\ valid_view_output y1 w1 /\ valid_view_output y2 w2
-      /\ valid_circuit c'
-      /\ size c' = size w1 - 1 /\ size w1 = size w2 /\ verify (w1, k1) c1 /\ verify (w2,k2) c2] = 1%r =>
-  phoare[ZKBoo(Com).verify :
-      h = (c',y) /\ m = (y1,y2,y3,c1,c2,c3) /\ z = (k2', w2', k3, w3) ==>
-      res /\ valid_output_shares y y1 y2 y3 /\ valid_view 2 w2' w3 c' k2' k3 /\ valid_view_output y2 w2' /\ valid_view_output y3 w3
-      /\ valid_circuit c'
-      /\ size c' = size w2' - 1 /\ size w2' = size w3 /\ verify (w2', k2') c2 /\ verify (w3, k3) c3] = 1%r =>
-  phoare[ZKBoo(Com).verify :
-      h = (c',y) /\ m = (y1,y2,y3,c1,c2,c3) /\ z = (k3', w3', k1', w1') ==>
-      res /\ valid_output_shares y y1 y2 y3 /\ valid_view 3 w3' w1' c' k3' k1' /\ valid_view_output y3 w3' /\ valid_view_output y1 w1'
-      /\ valid_circuit c'
-      /\ size c' = size w3' - 1 /\ size w3' = size w1' /\ verify (w3', k3') c3 /\ verify (w1', k1') c1] = 1%r =>
-  phoare[SoundnessInter.extract_views :
-      h = (c',y) /\ m = (y1,y2,y3,c1,c2,c3) /\ z1 = (k1, w1, k2, w2) /\ z2 = (k2', w2', k3, w3) /\ z3 = (k3', w3', k1', w1')
-      ==> res /\ (validate_response w1 w2 w3 w1' w2' w3' y y1 y2 y3 c' k1 k2 k3 k1' k2' k3')] = (1%r - binding_prob).
-proof.
-    move=> bg_ll accept1 accept2 accept3.
-    proc.
-    auto.
-    have Hcons := binding_three_cons_valid c1 c2 c3 (w1, k1) (w1', k1') (w2, k2) (w2', k2') (w3, k3) (w3', k3') bg_ll.
-    call Hcons. clear Hcons.
-    auto.
-    call accept3.
-    call accept2.
-    call accept1.
-    auto.
-    progress.
-    smt().
-    smt().
-    smt().
-    smt().
-    smt().
-    smt().
+  + progress.
     smt().
 qed.
-
-lemma zkboo_soundness_if_consistent
-      c' y y1 y2 y3 c1 c2 c3
-      k1' k2' k3' w1 w2 w3 &m:
-  phoare[ZKBoo(Com).witness_extractor :
-          valid_output_shares y y1 y2 y3
-          /\ valid_view 1 w1 w2 c' k1' k2'
-          /\ valid_view 2 w2 w3 c' k2' k3'
-          /\ valid_view 3 w3 w1 c' k3' k1'
-          /\ valid_view_output y1 w1
-          /\ valid_view_output y2 w2
-          /\ valid_view_output y3 w3
-          /\ size c' = size w1 - 1
-          /\ size w1 = size w2
-          /\ size w1 = size w3
-          /\ valid_circuit c' /\ h = (c',y) /\ a = (y1,y2,y3,c1,c2,c3) /\ z = [(k1', w1, k2', w2);(k2', w2, k3', w3);(k3', w3, k1', w1)]
-         ==> res <> None /\ R (c',y) (oget res)] = 1%r.
-proof.
-  proc.
-  auto.
-  rewrite /valid_output_share /valid_view_output; progress.
-  rewrite !oget_some.
-  clear H7 H8 H9 H10 H11 H12.
-  rewrite /R /R_DL.
-  progress.
-  rewrite /valid_output_shares in H.
-  rewrite /valid_view in H0.
-  rewrite /valid_view in H1.
-  rewrite /valid_view in H2.
-  have H' := eval_circuit_module c' [oget (onth w1 0) + oget (onth w2 0) + oget (onth w3 0)] y &m.
-  apply H'. clear H'.
-  have <- :
-    Pr[Phi.main(oget (onth w1 0) + oget (onth w2 0) + oget (onth w3 0), c') @ &m :
-      res = y] =
-    Pr[Circuit.eval(c', [oget (onth w1 0) + oget (onth w2 0) + oget (onth w3 0)]) @ &m :
-      res = y].
-  byequiv correctness_module=>//.
-  have -> :
-    Pr[Phi.main(oget (onth w1 0) + oget (onth w2 0) + oget (onth w3 0), c') @ &m :
-      res = y] =
-    Pr[Phi.main_fixed_input_and_tape(oget (onth w1 0), oget (onth w2 0), oget (onth w3 0), c' , k1', k2', k3') @ &m :
-      res = y].
-  byequiv main_fixed_equiv=>//.
-  rewrite H.
-  byphoare(: valid_circuit c' /\ c = c' /\ k1 = k1' /\ k2 = k2' /\ k3 = k3' /\ x1 = (oget (onth w1 0)) /\ x2 = (oget (onth w2 0)) /\ x3 = (oget (onth w3 0)) ==> res = last 0 w1 + last 0 w2 + last 0 w3)=>//.
-  proc.
-  inline Phi.reconstruct Phi.output.
-  wp.
-  inline *.
-  auto.
-    while (
-      size w10 = size w1 - size c0 /\
-         size w20 = size w2 - size c0 /\
-         size w30 = size w3 - size c0 /\
-         size c' = size c0 + size w10 - 1 /\
-         k10 = k1' /\
-         k20 = k2' /\
-         k30 = k3' /\
-         0 < size w10 /\
-         0 < size w20 /\
-         0 < size w30 /\
-         (forall i, 0 <= i < size c0 => (nth (ADDC(0,0)) c0 i = nth (ADDC(0,0)) c' (size w10 - 1 + i) /\ (size w10 -1 + i) < size c')) /\
-         (forall i, i < size w10 => nth 0 w1 i = nth 0 w10 i) /\
-         (forall i, i < size w20 => nth 0 w2 i = nth 0 w20 i) /\
-         (forall i, i < size w30 => nth 0 w3 i = nth 0 w30 i))
-        (size c0).
-  auto.
-  progress.
-  smt(size_rcons).
-  smt(size_rcons).
-  smt(size_rcons).
-  smt(size_rcons).
-  smt(size_rcons).
-  smt(size_rcons).
-  smt(size_rcons).
-  have H14' := H14 (i + 1) _. smt().
-  rewrite size_rcons.
-  have -> := nth_behead (ADDC(0,0)) c0{hr0} i _. smt().
-  smt.
-  smt(size_rcons).
-
-  rewrite !nth_rcons.
-  case (i < size w10{hr0});progress.
-  smt().
-  case (i = size w10{hr0}); progress.
-  have -> := H0 (size w10{hr0} - 1) _. smt.
-  have -> := ohead_head (ADDC(0,0)) c0{hr0} H18.
-  rewrite oget_some.
-  have <- : (nth (ADDC(0,0)) c' (size w10{hr0} - 1)) = head (ADDC(0,0)) c0{hr0}.
-  smt(nth0_head size_ge0).
-  rewrite /valid_circuit /valid_gate in H6.
-  have := H6 (size w10{hr0} - 1) _. smt.
-  have -> := onth_nth (ADDC(0,0)) c' (size w10{hr0} - 1). smt.
-  rewrite oget_some.
-  elim (nth (ADDC(0,0)) c' (size w10{hr0} - 1)); move=>x; case x=> x1 x2; smt().
-  smt(size_rcons head_behead).
-
-  rewrite !nth_rcons.
-  case (i < size w20{hr0});progress.
-  smt.
-  case (i = size w20{hr0}); progress.
-  have -> := H1 (size w20{hr0} - 1) _. smt.
-  have -> := ohead_head (ADDC(0,0)) c0{hr0} H18.
-  rewrite oget_some.
-  have <- : (nth (ADDC(0,0)) c' (size w20{hr0} - 1)) = head (ADDC(0,0)) c0{hr0}.
-  smt(nth0_head size_ge0).
-  rewrite /valid_circuit /valid_gate in H6.
-  have := H6 (size w20{hr0} - 1) _. smt.
-  have -> := onth_nth (ADDC(0,0)) c' (size w20{hr0} - 1). smt.
-  rewrite oget_some.
-  elim (nth (ADDC(0,0)) c' (size w20{hr0} - 1)); move=>x; case x=> x1 x2; smt().
-  smt(size_rcons head_behead).
-
-  rewrite !nth_rcons.
-  case (i < size w30{hr0});progress.
-  smt.
-  case (i = size w30{hr0}); progress.
-  have -> := H2 (size w30{hr0} - 1) _. smt.
-  have -> := ohead_head (ADDC(0,0)) c0{hr0} H18.
-  rewrite oget_some.
-  have <- : (nth (ADDC(0,0)) c' (size w30{hr0} - 1)) = head (ADDC(0,0)) c0{hr0}.
-  smt(nth0_head size_ge0).
-  rewrite /valid_circuit /valid_gate in H6.
-  have := H6 (size w30{hr0} - 1) _. smt.
-  have -> := onth_nth (ADDC(0,0)) c' (size w30{hr0} - 1). smt.
-  rewrite oget_some.
-  elim (nth (ADDC(0,0)) c' (size w30{hr0} - 1)); move=>x; case x=> x1 x2; smt().
-  smt(size_rcons head_behead).
-  smt(size_rcons head_behead).
-
-  auto.
-  smt(onth_nth oget_some size_ge0 dinput_ll nth_out nth_last).
-qed.
-
-
-local lemma zkboo_inter_soundness
-    c' y y1 y2 y3 c1 c2 c3
-    w1 w2 w3 w1' w2' w3'
-    k1 k2 k3 k1' k2' k3' &m:
-    islossless BindingGame(Com).bind_three =>
-    phoare[ZKBoo(Com).verify :
-        h = (c',y) /\ m = (y1,y2,y3,c1,c2,c3) /\ z = (k1, w1, k2, w2) ==>
-        res /\ valid_output_shares y y1 y2 y3 /\ valid_view 1 w1 w2 c' k1 k2 /\ valid_view_output y1 w1 /\ valid_view_output y2 w2
-        /\ valid_circuit c'
-        /\ size c' = size w1 - 1 /\ size w1 = size w2 /\ verify (w1, k1) c1 /\ verify (w2,k2) c2] = 1%r =>
-    phoare[ZKBoo(Com).verify :
-        h = (c',y) /\ m = (y1,y2,y3,c1,c2,c3) /\ z = (k2', w2', k3, w3) ==>
-        res /\ valid_output_shares y y1 y2 y3 /\ valid_view 2 w2' w3 c' k2' k3 /\ valid_view_output y2 w2' /\ valid_view_output y3 w3
-        /\ valid_circuit c'
-        /\ size c' = size w2' - 1 /\ size w2' = size w3 /\ verify (w2', k2') c2 /\ verify (w3, k3) c3] = 1%r =>
-    phoare[ZKBoo(Com).verify :
-        h = (c',y) /\ m = (y1,y2,y3,c1,c2,c3) /\ z = (k3', w3', k1', w1') ==>
-        res /\ valid_output_shares y y1 y2 y3 /\ valid_view 3 w3' w1' c' k3' k1' /\ valid_view_output y3 w3' /\ valid_view_output y1 w1'
-        /\ valid_circuit c'
-        /\ size c' = size w3' - 1 /\ size w3' = size w1' /\ verify (w3', k3') c3 /\ verify (w1', k1') c1] = 1%r =>
-    phoare[SoundnessInter.main :
-        h = (c',y) /\ m = (y1,y2,y3,c1,c2,c3) /\ z1 = (k1, w1, k2, w2) /\ z2 = (k2', w2', k3, w3) /\ z3 = (k3', w3', k1', w1')
-        ==> res] = (1%r - binding_prob).
-proof.
-  move=> bg_ll accept1 accept2 accept3.
-  (* phoare split (1%r - binding_prob) binding_prob : (validate_response w1 w2 w3 w1' w2' w3' y y1 y2 y3 c' k1 k2 k3 k1' k2' k3'). *)
-(*   proc. *)
-(*   seq 1 : (#pre /\ v /\ validate_response w1 w2 w3 w1' w2' w3' y y1 y2 y3 c' k1 k2 k3 k1' k2' k3') (1%r - binding_prob) 1%r binding_prob 0%r. *)
-(*   - auto. *)
-(*   - have H' := extraction_success c' y y1 y2 y3 c1 c2 c3 w1 w2 w3 w1' w2' w3' k1 k2 k3 k1' k2' k3' bg_ll accept1 accept2 accept3. *)
-(*     call H'. *)
-(*     auto. *)
-(*   wp. *)
-(*   have H' := zkboo_soundness_if_consistent c' y y1 y2 y3 c1 c2 c3 k1 k2 k3 w1 w2 w3 &m. *)
-(*   call H'. *)
-(*   skip. progress. *)
-(*   smt(). *)
-(*   smt(). *)
-(*   smt(). *)
-(*   smt(). *)
-(*   smt(). *)
-(*   smt(). *)
-(*   smt(). *)
-(*   smt(). *)
-(*   smt(). *)
-(*   smt(). *)
-(*   smt(). *)
-(*   smt(). *)
-(*   smt(). *)
-(*   smt(). *)
-(*   smt(). *)
-(*   smt(). *)
-(*   smt(). *)
-(*   smt(). *)
-(* hoare. *)
-(* inline *. auto. *)
-(* progress. *)
-(* smt(). *)
-
-(* lemma zkboo_soundness_if_consistent *)
-(*       c' y y1 y2 y3 c1 c2 c3 *)
-(*       k1' k2' k3' w1 w2 w3 &m: *)
-  have Hcons := binding_three_cons_valid c1 c2 c3 (w1, k1) (w1', k1') (w2, k2) (w2', k2') (w3, k3) (w3', k3') bg_ll.
-  proc.
-  inline SoundnessInter.ZK.witness_extractor.
-  auto.
-  inline SoundnessInter.extract_views.
-  (* call (: validate_response w1 w2 w3 w1' w2' w3' y y1 y2 y3 c' k1 k2 k3 k1' k2' k3'). *)
-
-
-  auto.
-  have Hcons := binding_three_cons_valid c1 c2 c3 (w1, k1) (w1', k1') (w2, k2) (w2', k2') (w3, k3) (w3', k3') bg_ll.
-  call Hcons. clear Hcons.
-  auto.
-  call accept3.
-  call accept2.
-  call accept1.
-  auto.
-  rewrite /valid_output_share /valid_view_output; progress.
-  rewrite !oget_some.
-  clear accept1 accept2 accept3 H25 H31 H32 H33 H34 H35 H36 H37 H26 H30 H8 H17 H20 H10 H19 H27 H24.
-  rewrite /R /R_DL.
-  progress.
-  rewrite /valid_output_shares in H0.
-  rewrite /valid_view in H1.
-  rewrite /valid_view in H18.
-  rewrite /valid_view in H9.
-  clear H29 H28 H15 H6 H14 H11 H21 H5.
-  have H' := eval_circuit_module c' [oget (onth w1' 0) + oget (onth w2' 0) + oget (onth w3' 0)] y &m.
-  apply H'. clear H'.
-  have <- :
-    Pr[Phi.main(oget (onth w1' 0) + oget (onth w2' 0) + oget (onth w3' 0), c') @ &m :
-      res = y] =
-    Pr[Circuit.eval(c', [oget (onth w1' 0) + oget (onth w2' 0) + oget (onth w3' 0)]) @ &m :
-      res = y].
-  byequiv correctness_module=>//.
-  have -> :
-    Pr[Phi.main(oget (onth w1' 0) + oget (onth w2' 0) + oget (onth w3' 0), c') @ &m :
-      res = y] =
-    Pr[Phi.main_fixed_input_and_tape(oget (onth w1' 0), oget (onth w2' 0), oget (onth w3' 0), c' , k1', k2', k3') @ &m :
-      res = y].
-  byequiv main_fixed_equiv=>//.
-  rewrite H0.
-  byphoare(: valid_circuit c' /\ c = c' /\ k1 = k1' /\ k2 = k2' /\ k3 = k3' /\ x1 = (oget (onth w1' 0)) /\ x2 = (oget (onth w2' 0)) /\ x3 = (oget (onth w3' 0)) ==> res = last 0 w1' + last 0 w2' + last 0 w3')=>//.
-  proc.
-  inline Phi.reconstruct Phi.output.
-  wp.
-  inline *.
-  auto.
-  while (size w10 = size w1' - size c0 /\
-         size w20 = size w2' - size c0 /\
-         size w30 = size w3' - size c0 /\
-         size c' = size c0 + size w10 - 1 /\
-         k10 = k1' /\
-         k20 = k2' /\
-         k30 = k3' /\
-         0 < size w10 /\
-         0 < size w20 /\
-         0 < size w30 /\
-         (forall i, 0 <= i < size c0 => (nth (ADDC(0,0)) c0 i = nth (ADDC(0,0)) c' (size w10 - 1 + i) /\ (size w10 -1 + i) < size c')) /\
-         (forall i, i < size w10 => nth 0 w1' i = nth 0 w10 i) /\
-         (forall i, i < size w20 => nth 0 w2' i = nth 0 w20 i) /\
-         (forall i, i < size w30 => nth 0 w3' i = nth 0 w30 i))
-        (size c0).
-  auto.
-  progress.
-  smt(size_rcons).
-  smt(size_rcons).
-  smt(size_rcons).
-  smt(size_rcons).
-  smt(size_rcons).
-  smt(size_rcons).
-  smt(size_rcons).
-  smt(nth_behead size_rcons).
-  smt(size_rcons).
-
-  rewrite !nth_rcons.
-  case (i < size w10{hr0}); first smt().
-  case (i = size w10{hr0}); progress.
-  have -> := H1 (size w10{hr0} - 1) _. smt(size_ge0).
-  have -> := ohead_head (ADDC(0,0)) c0{hr0} H24.
-  rewrite oget_some.
-  have <- : (nth (ADDC(0,0)) c' (size w10{hr0} - 1)) = head (ADDC(0,0)) c0{hr0}.
-  smt(nth0_head size_ge0).
-  rewrite /valid_circuit /valid_gate in H2.
-  have := H2 (size w10{hr0} - 1) _. smt(size_ge0).
-  have -> := onth_nth (ADDC(0,0)) c' (size w10{hr0} - 1). smt(size_ge0).
-  rewrite oget_some.
-  elim (nth (ADDC(0,0)) c' (size w10{hr0} - 1)); move=>x; case x=> x1 x2; smt().
-  smt(size_rcons head_behead).
-
-  rewrite !nth_rcons.
-  case (i < size w20{hr0}); first smt().
-  case (i = size w20{hr0}); progress.
-  have -> := H9 (size w20{hr0} - 1) _. smt(size_ge0).
-  have -> := ohead_head (ADDC(0,0)) c0{hr0} H24.
-  rewrite oget_some.
-  have <- : (nth (ADDC(0,0)) c' (size w20{hr0} - 1)) = head (ADDC(0,0)) c0{hr0}.
-  smt(nth0_head size_ge0).
-  rewrite /valid_circuit /valid_gate in H2.
-  have := H2 (size w20{hr0} - 1) _. smt(size_ge0).
-  have -> := onth_nth (ADDC(0,0)) c' (size w20{hr0} - 1). smt(size_ge0).
-  rewrite oget_some.
-  elim (nth (ADDC(0,0)) c' (size w20{hr0} - 1)); move=>x; case x=> x1 x2; smt().
-  smt(size_rcons head_behead).
-
-  rewrite !nth_rcons.
-  case (i < size w30{hr0}); first smt().
-  case (i = size w30{hr0}); progress.
-  have -> := H18 (size w30{hr0} - 1) _. smt(size_ge0).
-  have -> := ohead_head (ADDC(0,0)) c0{hr0} H24.
-  rewrite oget_some.
-  have <- : (nth (ADDC(0,0)) c' (size w30{hr0} - 1)) = head (ADDC(0,0)) c0{hr0}.
-  smt(nth0_head size_ge0).
-  rewrite /valid_circuit /valid_gate in H2.
-  have := H2 (size w30{hr0} - 1) _. smt(size_ge0).
-  have -> := onth_nth (ADDC(0,0)) c' (size w30{hr0} - 1). smt(size_ge0).
-  rewrite oget_some.
-  elim (nth (ADDC(0,0)) c' (size w30{hr0} - 1)); move=>x; case x=> x1 x2; smt().
-  smt(size_rcons head_behead).
-  smt().
-
-  auto.
-  smt(onth_nth oget_some size_ge0 dinput_ll nth_out nth_last).
-  smt(nth_last).
-  smt(nth_last).
-  smt(nth_last).
-  smt(nth_last).
-  smt(nth_last).
-  smt(nth_last).
-qed.
-
-
-lemma zkboo_soundness
-    c' y y1 y2 y3 c1 c2 c3
-    w1 w2 w3 w1' w2' w3'
-    k1 k2 k3 k1' k2' k3' &m:
-    islossless BindingGame(Com).bind_three =>
-    phoare[ZKBoo(Com).verify :
-        h = (c',y) /\ m = (y1,y2,y3,c1,c2,c3) /\ z = (k1, w1, k2, w2) ==>
-        res /\ valid_output_shares y y1 y2 y3 /\ valid_view 1 w1 w2 c' k1 k2 /\ valid_view_output y1 w1 /\ valid_view_output y2 w2
-        /\ valid_circuit c'
-        /\ size c' = size w1 - 1 /\ size w1 = size w2 /\ verify (w1, k1) c1 /\ verify (w2,k2) c2] = 1%r =>
-    phoare[ZKBoo(Com).verify :
-        h = (c',y) /\ m = (y1,y2,y3,c1,c2,c3) /\ z = (k2', w2', k3, w3) ==>
-        res /\ valid_output_shares y y1 y2 y3 /\ valid_view 2 w2' w3 c' k2' k3 /\ valid_view_output y2 w2' /\ valid_view_output y3 w3
-        /\ valid_circuit c'
-        /\ size c' = size w2' - 1 /\ size w2' = size w3 /\ verify (w2', k2') c2 /\ verify (w3, k3) c3] = 1%r =>
-    phoare[ZKBoo(Com).verify :
-        h = (c',y) /\ m = (y1,y2,y3,c1,c2,c3) /\ z = (k3', w3', k1', w1') ==>
-        res /\ valid_output_shares y y1 y2 y3 /\ valid_view 3 w3' w1' c' k3' k1' /\ valid_view_output y3 w3' /\ valid_view_output y1 w1'
-        /\ valid_circuit c'
-        /\ size c' = size w3' - 1 /\ size w3' = size w1' /\ verify (w3', k3') c3 /\ verify (w1', k1') c1] = 1%r =>
-    Pr[Sigma.SpecialSoundness(ZKBoo(Com)).main((c',y), (y1,y2,y3,c1,c2,c3), [1;2;3], [(k1, w1, k2, w2); (k2', w2', k3, w3); (k3', w3', k1', w1')]) @ &m :res]
-        = (1%r - binding_prob).
-proof.
-  move=> bg_ll accept1 accept2 accept3.
-  have -> :
-    Pr[SpecialSoundness(ZKBoo(Com)).main((c', y), (y1, y2, y3, c1, c2, c3), [1; 2; 3], [(k1, w1, k2, w2); (k2', w2', k3, w3); (k3', w3', k1', w1')]) @ &m : res] =
-    Pr[SoundnessInter.main((c', y), (y1, y2, y3, c1, c2, c3), (k1, w1, k2, w2), (k2', w2', k3, w3), (k3', w3', k1', w1') ) @ &m : res].
-  byequiv soundness_inter=>//.
-
-  byphoare(: h = (c',y) /\ m = (y1,y2,y3,c1,c2,c3) /\ z1 = (k1, w1, k2, w2) /\ z2 = (k2', w2', k3, w3) /\ z3 = (k3', w3', k1', w1') ==> _)=>//.
-  proc*.
-  have Hsuccess := zkboo_inter_soundness c' y y1 y2 y3 c1 c2 c3 w1 w2 w3 w1' w2' w3' k1 k2 k3 k1' k2' k3' &m bg_ll accept1 accept2 accept3.
-  call Hsuccess.
-  skip. progress.
-qed.
-
 
 end section Protocol.
